append and compose lemmas

src/computational_monads/simulation_semantics/oracle_append.lean
@@ -15,10 +15,9 @@ def oracle_append (so : simulation_oracle spec spec'')
   simulation_oracle (spec ++ spec') spec'' :=
 { S := so.S × so'.S,
   default_state := (so.default_state, so'.default_state),
-  o := λ i, match i with
-  | sum.inl i := λ ⟨t, s⟩, do { ⟨u, s'⟩ ← so.o i ⟨t, s.1⟩, pure (u, s', s.2) }
-  | sum.inr i := λ ⟨t, s⟩, do { ⟨u, s'⟩ ← so'.o i ⟨t, s.2⟩, pure (u, s.1, s') }
-  end }
+  o := λ i, sum.rec_on i
+    (λ i, λ x, do { u_s' ← so.o i ⟨x.1, x.2.1⟩, pure (u_s'.1, u_s'.2, x.2.2) })
+    (λ i, λ x, do { u_s' ← so'.o i ⟨x.1, x.2.2⟩, pure (u_s'.1, x.2.1, u_s'.2) }) }
 
 notation so `⟪++⟫` so' := oracle_append so so'
 
@@ -30,15 +29,25 @@ variables (so : simulation_oracle spec spec'') (so' : simulation_oracle spec' sp
 lemma default_state_oracle_append : (so ⟪++⟫ so').default_state =
   (so.default_state, so'.default_state) := rfl
 
+lemma oracle_append_apply_index (i : spec.ι ⊕ spec'.ι) : (so ⟪++⟫ so').o i = sum.rec_on i
+  (λ i, λ x, do { u_s' ← so.o i ⟨x.1, x.2.1⟩, pure (u_s'.1, u_s'.2, x.2.2) })
+  (λ i, λ x, do { u_s' ← so'.o i ⟨x.1, x.2.2⟩, pure (u_s'.1, x.2.1, u_s'.2) }) := rfl
+
 @[simp]
 lemma oracle_append_apply_inl : (so ⟪++⟫ so').o (sum.inl i) (t, s) =
-  so.o i (t, s.1) >>= λ ⟨u, s'⟩, pure (u, s', s.2) :=
-begin
-  simp [oracle_append],
-  sorry
-end
+  do { u_s' ← so.o i ⟨t, s.1⟩, pure (u_s'.1, u_s'.2, s.2) } := rfl
 
--- @[simp]
--- lemma simulate_oracle_append_pure : simulate (so ⟪++⟫ so') (pure a) s ≃ₚ
+@[simp]
+lemma oracle_append_apply_inr : (so ⟪++⟫ so').o (sum.inr i') (t', s) =
+  do { u_s' ← so'.o i' ⟨t', s.2⟩, pure (u_s'.1, s.1, u_s'.2)} := rfl
+
+section simulate
+
+variable [spec''.finite_range]
+
+lemma simulate_oracle_append_pure : simulate (so ⟪++⟫ so') (pure a) s ≃ₚ
+  (pure (a, s) : oracle_comp spec'' _) := rfl
+
+end simulate
 
 end oracle_append
